tla-tree/CrashSafeTreeInv.dfy
@@ -3,10 +3,9 @@ include "CrashSafeTree.dfy"
 module CrashSafeTreeInv {
 import opened CrashSafeTree
 
-predicate IsNodeStorage(lba:LBA, super:Sector)  // Trigger target.
-    requires super.Superblock?
+predicate IsNodeStorage(lba:LBA, virgin:int)  // Trigger target.
 {
-    1 <= lba < super.virgin
+    1 <= lba < virgin
 }
 
 predicate MinimalDisk(k:Constants)
@@ -14,17 +13,40 @@ predicate MinimalDisk(k:Constants)
     2 <= k.disk.size
 }
 
-predicate DiskStructureInv(k:Constants, s:Variables)
+predicate UsedSpaceFitsOnDisk(k:Constants, s:Variables, virgin:int)
     requires TreeDisk.WF(k.disk, s.disk)
     requires MinimalDisk(k)
 {
+    virgin <= k.disk.size
+}
+
+predicate IsNotSuperblock(k:Constants, s:Variables, virgin:int, lba:LBA)    // Trigger target
+    requires TreeDisk.WF(k.disk, s.disk)
+    requires MinimalDisk(k)
+    requires UsedSpaceFitsOnDisk(k, s, virgin)
+    requires IsNodeStorage(lba, virgin)
+{
+    !TreeDisk.PeekF(k.disk, s.disk, lba).Superblock?
+}
+
+predicate StorageIsNotSuperblocks(k:Constants, s:Variables, virgin:int)
+    requires TreeDisk.WF(k.disk, s.disk)
+    requires MinimalDisk(k)
+    requires UsedSpaceFitsOnDisk(k, s, virgin)
+{
+    forall lba :: IsNodeStorage(lba, virgin) ==> IsNotSuperblock(k, s, virgin, lba)
+}
+
+predicate DiskStructureInv(k:Constants, s:Variables)
+{
+    && TreeDisk.WF(k.disk, s.disk)
+    && MinimalDisk(k)
+
     && 1 <= k.disk.size // Gotta have room for a superblock!
     && var super := TreeDisk.PeekF(k.disk, s.disk, SUPERBLOCK_LBA());
     && super.Superblock?
-    && super.virgin <= k.disk.size   // used blocks fit on the disk
-    && (forall lba :: IsNodeStorage(lba, super) ==>
-            !TreeDisk.PeekF(k.disk, s.disk, lba).Superblock?
-        )
+    && UsedSpaceFitsOnDisk(k, s, super.virgin)
+    && StorageIsNotSuperblocks(k, s, super.virgin)
 }
 
 predicate CacheEntryReflectsDisk(k:Constants, s:Variables, lba:LBA)
@@ -41,24 +63,49 @@ predicate CacheReflectsDisk(k:Constants, s:Variables)
     forall lba :: lba in s.cache ==> CacheEntryReflectsDisk(k, s, lba)
 }
 
+predicate VirginExcludesSuperblock(k:Constants, s:Variables)
+    requires DiskStructureInv(k, s) // get a well-formed, nonempty disk
+{
+    && var super := TreeDisk.PeekF(k.disk, s.disk, SUPERBLOCK_LBA());
+    && 2 <= super.virgin
+}
+
 predicate Inv(k:Constants, s:Variables)
 {
     && TreeDisk.WF(k.disk, s.disk)
     && MinimalDisk(k)
     && DiskStructureInv(k, s)
     && CacheReflectsDisk(k, s)
+    && VirginExcludesSuperblock(k, s)
+}
+
+lemma CanAllocateImpliesNotSuperblock(k:Constants, s:Variables, super:Sector, childRead:NRead)
+    requires Inv(k, s)
+    requires CanAllocate(k, s, super, childRead)
+    ensures childRead.lba != SUPERBLOCK_LBA();
+{
+    if NodeDisconnected(k, s, childRead) {
+        assert childRead.lba != SUPERBLOCK_LBA();
+    } else if NodeIsCold(k, s, childRead.lba, TreeDisk.NodeSector(childRead.node)) {
+        assert childRead.lba != SUPERBLOCK_LBA();
+    } else {
+        assert SectorIsVirgin(k, s, super, childRead.lba);
+        assert childRead.lba != SUPERBLOCK_LBA();
+    }
 }
 
 lemma InvHoldsInit(k:Constants, s:Variables)
     requires Init(k, s)
     ensures Inv(k, s)
 {
+/*
     var super := TreeDisk.PeekF(k.disk, s.disk, SUPERBLOCK_LBA());
-    forall lba | IsNodeStorage(lba, super)
+    forall lba | IsNodeStorage(lba, super.virgin)
         ensures !TreeDisk.PeekF(k.disk, s.disk, lba).Superblock?
     {
         assert lba == 1;
     }
+*/
 }
 
 lemma InvHoldsInduction(k:Constants, s:Variables, s':Variables)
@@ -74,7 +121,9 @@ lemma InvHoldsInduction(k:Constants, s:Variables, s':Variables)
         case CacheEvictActionStep(lba) => {
             assert DiskStructureInv(k, s');
         }
-        case PrepareGrowActionStep(parentRead, i, childRead) => {
+        case PrepareGrowActionStep(super, parentRead, i, childRead) => {
+            assert WriteThroughNode(k, s, s', childRead.lba, ChildNodeForParentIdx(parentRead, i));
+            assert childRead.lba != SUPERBLOCK_LBA();
             assert DiskStructureInv(k, s');
         }
         case CommitGrowActionStep(parentRead, i, childRead) => {
@@ -91,10 +140,24 @@ lemma InvHoldsInduction(k:Constants, s:Variables, s':Variables)
         case DeleteActionStep(datum, lookup) => {
             assert DiskStructureInv(k, s');
         }
-        case MoveToFreeListActionStep(lba, childRead) => {
+        case MoveToFreeListActionStep(childRead) => {
             assert DiskStructureInv(k, s');
         }
         case CommitFreeListActionStep(super) => {
+        /*
+            forall lba | IsNodeStorage(lba, super.virgin)
+                ensures IsNotSuperblock(k, s', super.virgin, lba)
+            {
+            }
+            assert StorageIsNotSuperblocks(k, s', super.virgin);
+            assert DiskStructureInv(k, s');
+            */
+        }
+        case WriteAnythingIntoVirginActionStep(super, lba, data) => {
+        }
+        case ExpandStorageActionStep(super, newVirgin, nreads) => {
+            assert UsedSpaceFitsOnDisk(k, s', newVirgin);
+            assert StorageIsNotSuperblocks(k, s', newVirgin);
             assert DiskStructureInv(k, s');
         }
     }
